WIP Make address concrete

Systems/Address.v
@@ -1,5 +1,5 @@
 From mathcomp.ssreflect
-Require Import ssreflect eqtype fintype.
+Require Import ssreflect ssrnat ssrfun eqtype choice fintype ssrbool seq.
 From fcsl
 Require Import ordtype.
 
@@ -9,12 +9,36 @@ Require Import ordtype.
         https://github.com/coq/coq/issues/4749
  *)
 Module Type NetAddr.
-(* Address is an IP:port pair or something similar *)
 (* Needs to be finType because the global state is map from Address ->
    State and _all_ addresses (i.e. need to be able to enumerate them)
-   should start with the initial state.
-*)
-Parameter Address : finType.
-Definition Address_ordMixin := fin_ordMixin Address.
+   should start with the initial state. *)
+Structure Address: Type := mkAddr {
+    ip: 'I_2*'I_2*'I_2*'I_2;
+    port:'I_2
+}.
+
+Definition prod_of_address e :=
+let: mkAddr ipv4 portNum := e in (ipv4, portNum).
+
+Definition address_of_prod p :=
+let: (ipv4, portNum) := p in mkAddr ipv4 portNum.
+
+Lemma prod_of_addressK : cancel prod_of_address address_of_prod.
+Proof. by case. Qed.
+
+Definition address_eqMixin := CanEqMixin prod_of_addressK.
+Canonical Address_eqType := Eval hnf in EqType Address address_eqMixin.
+
+Definition address_choiceMixin := CanChoiceMixin prod_of_addressK.
+Canonical Address_choiceType := Eval hnf in ChoiceType Address address_choiceMixin.
+
+Definition address_countMixin := CanCountMixin prod_of_addressK.
+Canonical Address_countType := Eval hnf in CountType Address address_countMixin.
+
+Definition address_finMixin := CanFinMixin prod_of_addressK.
+Canonical Address_finType := Eval hnf in FinType Address address_finMixin.
+
+Definition Address_ordMixin := fin_ordMixin [finType of Address].
 Canonical Address_ordType := Eval hnf in OrdType Address Address_ordMixin.
+
 End NetAddr.
